% \title{
% Orbit-Stabilizer Theorem
% }

% Scribe: Fred Zhang

% Date: Monday, May 6, 2019

\subsection{Orbits and Stabilizers}

Given $s \in S$ and $G$ a permutation group acting on $S$.

\begin{definition}
    $\text{orbit}(s) = \set{ \pi s \mid \pi \in G }$
\end{definition}

\begin{definition}
    $\text{stabilizer}(s) = \set{ \pi \in G  \mid \pi s = s }$
\end{definition}

\begin{theorem}1
    Orbit-Stabilizer Theorem: For all $s \in S$ and $G$ acting on $S$, $|\text{orbit}(s)| \cdot |\text{stabilizer}(s)| = |G|$
\end{theorem}

$\text{stabilizer}(s)$ is a subgroup of $G$, so by Lagrange's theorem, $|\text{stabilizer}(s)| \mid |G|$

\begin{lemma}1
    If $\pi \in G$ and $\pi \in \text{stabilizer}(s)$, then $\pi^{-1} s=s$.
\end{lemma}
\begin{proof}
    \begin{align*}
        s &= \pi s \\ 
        \pi^{-1} s &= \pi^{-1} \pi s \\ 
        \pi^{-1} s &= s
    \end{align*}
\end{proof}

So now the orbit of $S$ forms cosets of $\text{stabilizer}(s)$ (there is a 1-1 corespondence). 
So $|\text{orbit}(s)| = $ \# of cosets of $\text{stabilizer}(s)$. Applying Lagrange's theorem
gives the orbit-stabilizer theorem.